compiler/wasm/wasm_ast.ml
@@ -7,7 +7,7 @@ let eval j w env =
   (* let res = Wasm_engine.invoke inst arg in *)
   (* Some res *)
 
-let imp_ejson_to_wasm_ast fe fer i = Wasm_translate.imp i
+let imp_ejson_to_wasm_ast i = Wasm_translate.imp i
 let to_string q =
   let sexpr = Wasm.Arrange.module_ q in
   Wasm.Sexpr.to_string 72 sexpr
