compiler/wasm/wasm_ast.mli
@@ -5,5 +5,5 @@ open ImpEJson
 
 type t = Wasm.Ast.module_
 val eval : (char list * char list) list -> t -> 'a jbindings -> ('a ejson) option
-val imp_ejson_to_wasm_ast : 'a foreign_ejson -> 'a foreign_ejson_runtime -> 'a imp_ejson -> t
+val imp_ejson_to_wasm_ast : ('a,'b) imp_ejson -> t
 val to_string : t -> string
