compiler/core/Driver/CompCustom.v
@@ -113,7 +113,8 @@ Section CompCustom.
   Context {fruntime:foreign_runtime}.
   Context {foreign_ejson_model:Set}.
   Context {fejson:foreign_ejson foreign_ejson_model}.
-  Context {ftejson:foreign_to_ejson}.
+  Context {foreign_ejson_runtime_op : Set}.
+  Context {ftejson:foreign_to_ejson foreign_ejson_model foreign_ejson_runtime_op}.
   Context {frtejson:foreign_to_ejson_runtime}.
   Context {fredop:foreign_reduce_op}.
   Context {ftoredop:foreign_to_reduce_op}.
