compiler/core/Imp/Lang/ImpEJsonSize.v
@@ -25,18 +25,19 @@ Require Import ImpEJson.
 Section ImpEJsonSize.
   Context {foreign_ejson_model:Set}.
   Context {fejson:foreign_ejson foreign_ejson_model}.
-  Context {fejruntime:foreign_ejson_runtime}.
+  Context {foreign_ejson_runtime_op : Set}.
+  Context {fejruntime:foreign_ejson_runtime foreign_ejson_runtime_op}.
 
-  Definition imp_ejson_expr_size (e:imp_ejson_expr) : nat :=
+  Definition imp_ejson_expr_size (e:@imp_ejson_expr foreign_ejson_model foreign_ejson_runtime_op) : nat :=
     imp_expr_size e.
 
-  Definition imp_ejson_stmt_size (stmt:imp_ejson_stmt) : nat :=
+  Definition imp_ejson_stmt_size (stmt:@imp_ejson_stmt foreign_ejson_model foreign_ejson_runtime_op) : nat :=
     imp_stmt_size stmt.
 
-  Definition imp_ejson_function_size (q:imp_ejson_function) : nat :=
+  Definition imp_ejson_function_size (q:@imp_ejson_function foreign_ejson_model foreign_ejson_runtime_op) : nat :=
     imp_function_size q.
 
-  Fixpoint imp_ejson_size (q: imp_ejson) : nat :=
+  Fixpoint imp_ejson_size (q: @imp_ejson foreign_ejson_model foreign_ejson_runtime_op) : nat :=
     imp_size q.
 
 End ImpEJsonSize.
